Remove extra sizeof_dtyp in serialization.

src/coq/Handlers/Serialization.v
@@ -80,33 +80,6 @@ Module Make(Addr:MemoryAddress.ADDRESS)(LLVMIO: LLVM_INTERACTIONS(Addr))(SIZEOF:
   Definition sbytes_of_int (e : Endianess) (count:nat) (z:Z) : list SByte :=
     List.map Byte (bytes_of_int e count z). *)
 
-    (** ** Size of a dynamic type
-      Computes the byte size of a [dtyp]. *)
-    Fixpoint sizeof_dtyp (ty:dtyp) : N :=
-      match ty with
-      | DTYPE_I 1          => 1 (* TODO: i1 sizes... *)
-      | DTYPE_I 8          => 1
-      | DTYPE_I 32         => 4
-      | DTYPE_I 64         => 8
-      | DTYPE_I _          => 0 (* Unsupported integers *)
-      | DTYPE_IPTR         => N.of_nat ptr_size
-      | DTYPE_Pointer      => N.of_nat ptr_size
-      | DTYPE_Packed_struct l
-      | DTYPE_Struct l     => fold_left (fun acc x => (acc + sizeof_dtyp x)%N) l 0%N
-      | DTYPE_Vector sz ty'
-      | DTYPE_Array sz ty' => sz * sizeof_dtyp ty'
-      | DTYPE_Float        => 4
-      | DTYPE_Double       => 8
-      | DTYPE_Half         => 4
-      | DTYPE_X86_fp80     => 10 (* TODO: Unsupported, currently modeled by Float32 *)
-      | DTYPE_Fp128        => 16 (* TODO: Unsupported, currently modeled by Float32 *)
-      | DTYPE_Ppc_fp128    => 16 (* TODO: Unsupported, currently modeled by Float32 *)
-      | DTYPE_Metadata     => 0
-      | DTYPE_X86_mmx      => 8 (* TODO: Unsupported *)
-      | DTYPE_Opaque       => 0 (* TODO: Unsupported *)
-      | _                  => 0 (* TODO: add support for more types as necessary *)
-      end.
-
     Definition uvalue_bytes_little_endian (uv :  uvalue) (dt : dtyp) (sid : store_id) : list uvalue
       := map (fun n => UVALUE_ExtractByte uv dt (UVALUE_IPTR (Z.of_N n)) sid) (Nseq 0 ptr_size).
  
@@ -1320,9 +1293,8 @@ Proof.
                 end
               ].
   - inv SUP; exfalso; apply H; constructor.
-  - inv SIZE.
+  - rewrite sizeof_dtyp_void in SIZE. inv SIZE.
 Qed.
-
 
 Section ConcretizeInductive.
 
